thy/LOFT/Examples/SQRL/akachan.py
@@ -1,0 +1,206 @@
+#!/usr/bin/python
+
+from mininet.net import Mininet
+from mininet.topo import Topo
+from mininet.link import TCLink
+from mininet.cli import CLI
+from mininet.util import quietRun
+from mininet.log import setLogLevel, info, output, debug, error
+from mininet.term import makeTerms
+from mininet.node import Host, OVSBridge, OVSSwitch
+from mininet.util import waitListening
+
+from random import randint
+from sys import exit, stdin, argv
+from re import findall
+from time import sleep
+import os
+import struct, socket
+
+ip2int = lambda ipstr: struct.unpack('!I', socket.inet_aton(ipstr))[0]
+int2ip = lambda n: socket.inet_ntoa(struct.pack('!I', n))
+
+def pne(s):
+	if not s.strip() == "":
+		if not "\n" in s:
+			s = s + "\n"
+		print(s)
+
+def qcall(o,a,*args):
+	info('config {}: {}\n'.format(o, args))
+	orv = a(*args)
+	rv = orv
+	if not rv.strip() == "":
+		if not "\n" in rv:
+			rv = rv + "\n"
+		error('{} in {} failed: {}'.format(args, o, rv))
+	return orv
+
+class IFCHlp:
+	ifcs = [
+		('ldit', ("10.13.42.137", 29)),
+		('lmd', ("10.13.42.129", 29)),
+		('loben', ("10.13.42.145", 28)),
+		('lup', ("13.14.15.58", 24)),
+		('vocb', ("10.13.43.17", 28)),
+		('vpriv', ("10.13.37.200", 24)),
+		('vshit', ("10.13.43.1", 28)),
+		('wg', ("10.13.41.1", 27)),
+		('wt', ("10.13.42.161", 28)),
+	] # the order is important. the port numbers will be assigned based on it! (yes, I got it wrong at some point. take a good hard look.)
+
+	def ifc(self):
+		for (iface, ipsn) in self.ifcs:
+			self.intf('s1-' + iface).setIP(*ipsn)
+
+class StaticSwitch(OVSSwitch,IFCHlp): # Bridge is closest to what we want. It quacks like it.
+	batch = False
+	requirecommonnet=True
+	@classmethod
+	def addSelf(cls, name, topo):
+		return topo.addSwitch(name, ip=None, cls=StaticSwitch)
+	@classmethod
+	def batchStartup(cls, switches, *_parm, **_parms):
+		rv = OVSSwitch.batchStartup(switches, *_parm, **_parms)
+		for s in switches:
+			s.poststart()
+		return rv
+	def poststart(self):
+		self.ifc()
+		flows = [
+			"'table=0,hard_timeout=0,idle_timeout=0,priority=1,action=drop'",
+			"'table=0,hard_timeout=0,idle_timeout=0,priority=2,arp,action=flood'",
+			"'table=0,hard_timeout=0,idle_timeout=0,priority=2,ip,ct_state=-trk,action=ct(table=1,zone=42)'",
+
+			"'table=1,hard_timeout=0,idle_timeout=0,priority=2,ip,ct_state=+trk+new,action=goto_table:2'",
+			"'table=1,hard_timeout=0,idle_timeout=0,priority=2,ip,ct_state=+trk+est,action=goto_table:3'",
+			"'table=1,hard_timeout=0,idle_timeout=0,priority=1,action=drop'",
+		]
+		with open('sqrl_of_new.txt') as f:
+			    for line in f:
+					line = line.replace('action=output', 'action=ct(commit,zone=42),output') # cheating!
+					line = line.replace('\n', "'")
+					flows.append("'table=2," + line);
+		with open('sqrl_of_est.txt') as f:
+			    for line in f:	
+					line = line.replace('\n', "'")
+					flows.append("'table=3," + line);
+		for f in flows:
+			qcall(self,self.dpctl,"add-flow", f)
+
+class DRtr(Host,IFCHlp):
+	requirecommonnet=False
+	@classmethod
+	def addSelf(cls, name, topo):
+		return topo.addHost(name, ip=None, cls=DRtr)
+	def config(self, *_parm, **_params):
+		rv = Host.config(self, *_parm, **_params)
+		qcall(self,self.cmd, "sed <iptables-save 's/-i /-i s1-/; s/-o /-o s1-/;' | iptables-restore")
+		self.ifc()
+		self.cmd('sysctl -w net.ipv4.ip_forward=1')
+		return rv
+	def terminate(self):
+		self.cmd('sysctl net.ipv4.ip_forward=0')
+		Host.terminate(self)
+
+class DTopo(Topo):
+	"""Topology for Test:
+	   client - router - internet (actually, the internet is just a single box...)"""
+	def __init__(self, scls):
+		self.scls = scls
+		return Topo.__init__(self)
+	def build(self):
+		commonnet = None;
+		if self.scls.requirecommonnet:
+			commonnet = '5'
+		switch = self.scls.addSelf('s1', topo=self)
+		for (iface, (ip, net)) in IFCHlp.ifcs:
+			name = 'h' + iface
+			mip = int2ip(ip2int(ip) + 1) # just assume that there's another IP in that net, directly next. Should fail soon if untrue...
+			mnet = commonnet or str(net)
+			dev = self.addHost(name, ip=mip+'/'+mnet, defaultRoute='via '+ip)
+			self.addLink(dev, switch, intfName2='s1-' + iface)
+		#client = self.addHost('h1', ip='10.0.1.2/'+net, defaultRoute='via 10.0.1.1')
+		#nhsl = self.addLink(nhost,  switch,  intfName2='s1-wan')
+
+def dump(ofile, strng):
+	with open(ofile, "w") as fo:
+		fo.write(strng.replace("\r\n","\n"))
+
+def tcpreachtest(net, client, server, port=80, timeout=2.5):
+	output("TCP {}: {} -> {}: ".format(port, client, server))
+	rand = "{}".format(randint(0,18446744073709551615))
+	server.sendCmd("socat EXEC:'echo {}' TCP4-LISTEN:{},reuseaddr".format(rand,port))
+	sleep(.1) # I doubt there is a way of knowing whether it is listening.
+	cliout = client.cmd("socat TCP:{}:{},connect-timeout={} -".format(server.IP(), port, timeout))
+	server.sendInt()
+	servout = server.waitOutput()
+	result = cliout.strip() == rand
+	output("{}\n".format("success" if result else "fail"))
+	debug("tcp test: socat server: {}".format(servout.strip()))
+	debug("tcp test: socat client: {}".format(cliout.strip()))
+	debug("tcp test:     expected: {}".format(rand))
+	return result
+
+def tcpreachtests(net, hosts, ports=[80], timeout=2.5):
+	if type(ports) is not list:
+		ports = [ports]
+	for port in ports:
+		for h1 in hosts:
+			for h2 in hosts:
+				if h1 == h2:
+					continue
+				tcpreachtest(net, h1, h2, port, timeout)
+
+def makearpentries(host, hosts):
+	# add all arp entries for host to hosts.
+	for intf in host.intfList():
+		if intf.MAC() and intf.IP(): # will also sort out loopback
+			for host in hosts:
+				host.cmd("arp -s {} {}".format(intf.IP(), intf.MAC())) # will fail with Netwok unreachable at given times. Easier to ignore than fix.
+
+def standalone():
+	if "debug" in argv:
+		setLogLevel( 'debug' )
+	elif "info" in argv:
+		setLogLevel( 'info' )
+	scls=None
+	if "of" in argv:
+		scls = StaticSwitch 
+	elif "lr" in argv:
+		scls = DRtr
+	else:
+		print("Supply either of (for OpenFlow) or lr (for a Linux Router)")
+		exit(-1)
+	topo = DTopo(scls=scls)
+	net = Mininet(topo=topo,autoSetMacs=True)
+	net.start()
+	sw = net.get('s1')
+	trabant = net.get(*['h' + ifce for ifce,_ in IFCHlp.ifcs])
+	if "noarp" not in argv:
+		makearpentries(sw, trabant)
+	#print(sw.cmd("netstat -tulpen"))
+	if "dump" in argv:
+		if "lr" in argv:
+			dump('iptables-save-dump', sw.cmd('iptables-save'))
+			dump('ip-route-dump', sw.cmd('ip route'))
+			dump('collectedmacs-dump', sw.cmd('collectmacs.sh'))
+	if "test" in argv:
+		net.ping(trabant)
+		tcpreachtests(net,trabant,ports=[80,22])
+		if "of" in argv and "dump" in argv:
+			info(sw.dpctl("dump-flows"));
+			for ln in sw.cmd("ovs-dpctl", "dump-conntrack").splitlines():
+				if "zone=42" in ln:
+					output(ln + '\n')
+	if "cli" in argv:
+		CLI(net)
+	net.stop()
+
+if __name__ == '__main__':
+	standalone()
+
+topos = { 
+	'lr': ( lambda: DTopo(scls=DRtr) ), 
+	'of': ( lambda: DTopo(scls=StaticSwitch) ),
+}
